new/proof/github_com/sanjit_bhat/pav/server_proof/server.v
@@ -1,39 +1,76 @@
 From New.generatedproof.github_com.sanjit_bhat.pav Require Import server.
-From New.proof.github_com.sanjit_bhat.pav Require Import prelude.
 
 From New.proof Require Import sync time.
 From New.proof.github_com.goose_lang Require Import std.
 From New.proof.github_com.sanjit_bhat.pav Require Import
   cryptoffi hashchain ktcore merkle.
 
+From New.proof.github_com.sanjit_bhat.pav Require Import prelude.
+
 Module server.
+
+(* gmap from uid's to list of pks (indexed by version). *)
+Definition keys_ty := gmap w64 (list $ list w8).
 
 Module state.
 Record t :=
   mk {
-    (* gmap from uid's to list of pks (indexed by version). *)
-    keys: gmap w64 (list $ list w8);
-    digs: list $ list w8;
+    (* pending map of all keys.
+    client gives server permission to add to this. *)
+    pending: keys_ty;
+    (* history of digs and keys.
+    server can update this by adding dig that corresponds to curr pending. *)
+    hist: list (list w8 * keys_ty);
   }.
 End state.
 
+Module serverγ.
+Record t :=
+  mk {
+    sig_pk: list w8;
+    vrf_pk: list w8;
+  }.
+End serverγ.
+
 Section proof.
 Context `{hG: heapGS Σ, !ffi_semantics _ _, !globalsGS Σ} {go_ctx : GoContext}.
-Context `{!pavG Σ}.
 
-Axiom Server_names : Type.
+Definition wish_checkMemb pk uid ver dig memb : iProp Σ :=
+  ∃ label mapVal,
+  let enc_label := ktcore.MapLabel.pure_enc (ktcore.MapLabel.mk' uid ver) in
+  let enc_val := ktcore.CommitOpen.pure_enc memb.(ktcore.Memb.PkOpen) in
+  "#His_vrf_proof" ∷ cryptoffi.is_vrf_proof pk enc_label memb.(ktcore.Memb.LabelProof) ∗
+  "#His_vrf_out" ∷ cryptoffi.is_vrf_out pk enc_label label ∗
+  "#His_mapVal" ∷ cryptoffi.is_hash (Some enc_val) mapVal ∗
+  "#Hwish_memb" ∷ merkle.wish_VerifyMemb label mapVal memb.(ktcore.Memb.MerkleProof) dig.
 
-(* Could put the sigPk into here. *)
-Implicit Types γ : Server_names.
+Definition wish_checkHist pk uid (prefixLen : w64) dig hist : iProp Σ :=
+  ([∗ list] ver ↦ memb ∈ hist,
+    wish_checkMemb pk uid (uint.Z prefixLen + ver) dig memb).
+
+Definition wish_checkNonMemb pk uid ver dig nonMemb : iProp Σ :=
+  ∃ label,
+  let enc := ktcore.MapLabel.pure_enc (ktcore.MapLabel.mk' uid ver) in
+  "#His_vrf_proof" ∷ cryptoffi.is_vrf_proof pk enc nonMemb.(ktcore.NonMemb.LabelProof) ∗
+  "#His_vrf_out" ∷ cryptoffi.is_vrf_out pk enc label ∗
+  "#Hwish_nonMemb" ∷ merkle.wish_VerifyNonMemb label nonMemb.(ktcore.NonMemb.MerkleProof) dig.
+
+Implicit Types γ : serverγ.t.
+Implicit Types σ : state.t.
 
 Axiom is_Server : ∀ (s : loc) γ, iProp Σ.
 
-Axiom own_Server : ∀ γ (σ : state.t), iProp Σ.
+Axiom own_Server : ∀ γ σ, iProp Σ.
 
 Axiom own_Server_timeless : ∀ γ σ,  Timeless (own_Server γ σ).
 Global Existing Instance own_Server_timeless.
 
-Axiom pure_put : w64 → list w8 → w64 → state.t → state.t.
+Definition pure_put σ uid pk (ver : w64) :=
+  let pks := σ.(state.pending) !!! uid in
+  (* drops put if not right version. *)
+  match bool_decide (uint.nat ver = length pks) with false => σ | _ =>
+  set state.pending (<[uid:=pks ++ [pk]]>) σ
+  end.
 
 (* RPC spec needs □ in front of atomic update. *)
 Lemma wp_Server_Put s γ uid pk sl_pk ver :
@@ -41,8 +78,8 @@ Lemma wp_Server_Put s γ uid pk sl_pk ver :
   is_Server s γ -∗
   sl_pk ↦*□ pk -∗
   □ (|={⊤,∅}=> ∃ σ, own_Server γ σ ∗
-    (own_Server γ (pure_put uid pk ver σ) ={∅,⊤}=∗
-      Φ #())) -∗
+    (own_Server γ (pure_put σ uid pk ver) ={∅,⊤}=∗ True)) ∗
+  Φ #() -∗
   WP s @ (ptrT.id server.Server.id) @ "Put" #uid #sl_pk #ver {{ Φ }}.
 Proof.
 Admitted.
@@ -53,15 +90,22 @@ Lemma wp_Server_History s γ (uid prevEpoch prevVerLen : w64) :
   ∀ Φ,
   is_Server s γ -∗
   (|={⊤,∅}=> ∃ σ, own_Server γ σ ∗ (own_Server γ σ ={∅,⊤}=∗
-    (* postcond. *)
-    ∃ (sl_chainProof sl_linkSig sl_hist : slice.t) (ptr_bound : loc) (err : ktcore.Blame),
+    (* postcond. it only references σ.(state.hist). *)
+    ∃ sl_chainProof sl_linkSig sl_hist ptr_bound (err : ktcore.Blame)
+      lastDig lastKeys lastLink,
+    let numEps := length σ.(state.hist) in
+    let pks := lastKeys !!! uid in
+    "%Hlast_hist" ∷ ⌜last σ.(state.hist) = Some (lastDig, lastKeys)⌝ ∗
+    "#His_lastLink" ∷ hashchain.is_chain σ.(state.hist).*1 None lastLink numEps ∗
     ((
       "%Herr" ∷ ⌜err = {[ ktcore.BlameUnknown ]}⌝ ∗
-      "%Hwish" ∷ ⌜uint.nat prevEpoch ≥ length σ.(state.digs) ∨
-        uint.nat prevVerLen > length (σ.(state.keys) !!! uid)⌝
+      "%Hwish" ∷ ⌜uint.nat prevEpoch ≥ length σ.(state.hist) ∨
+        uint.nat prevVerLen > length pks⌝
     ) ∨ (
       ∃ chainProof (linkSig : list w8) sl0_hist hist bound,
       "%Herr" ∷ ⌜err = ∅⌝ ∗
+      "%Hwish" ∷ ⌜uint.nat prevEpoch < length σ.(state.hist) ∧
+        uint.nat prevVerLen ≤ length pks⌝ ∗
 
       "#Hsl_chainProof" ∷ sl_chainProof ↦*□ chainProof ∗
       "#Hsl_linkSig" ∷ sl_linkSig ↦*□ linkSig ∗
@@ -71,8 +115,17 @@ Lemma wp_Server_History s γ (uid prevEpoch prevVerLen : w64) :
       "#Hptr_bound" ∷ ktcore.NonMemb.own ptr_bound bound (□) ∗
 
       "%Hwish_chainProof" ∷ ⌜hashchain.wish_Verify chainProof
-        (drop (S (uint.nat prevEpoch)) σ.(state.digs))⌝)) -∗
-      (* TODO: correctness preds should tie into σ. *)
+        (drop (S (uint.nat prevEpoch)) σ.(state.hist).*1)⌝ ∗
+      "#Hwish_linkSig" ∷ ktcore.wish_VerifyLinkSig γ.(serverγ.sig_pk)
+        (W64 $ (Z.of_nat numEps - 1)) lastLink linkSig ∗
+      "#Hwish_hist" ∷ wish_checkHist γ.(serverγ.vrf_pk) uid prevVerLen
+        lastDig hist ∗
+      "%Heq_hist" ∷ ⌜Forall2
+        (λ x y, x = y.(ktcore.Memb.PkOpen).(ktcore.CommitOpen.Val))
+        (drop (uint.nat prevVerLen) pks) hist⌝ ∗
+      "#Hwish_bound" ∷ wish_checkNonMemb γ.(serverγ.vrf_pk) uid
+        (W64 $ length pks) lastDig bound
+    )) -∗
     Φ #(sl_chainProof, sl_linkSig, sl_hist, ptr_bound, err))) -∗
   WP s @ (ptrT.id server.Server.id) @ "History" #uid #prevEpoch #prevVerLen {{ Φ }}.
 Proof.
